back to StAE.fst instead of .fsti, which is too painful to work with interactively

src/tls/StAE.fst
@@ -1,27 +1,89 @@
-module StAE
-
-(* Multiplexing between StatefulLHAE and StreaAE for the record layer *) 
-
+module StAE // See StAE.fsti
+open FStar.HyperHeap
 open FStar.Monotonic.RRef
-
+open FStar.Seq
 open Platform.Bytes
 
 open TLSConstants
 open TLSInfo
+open Content
+
+module HH = HyperHeap
+module MR = FStar.Monotonic.RRef
+// plaintexts are defined in Content.fragment i
+
+// ciphertexts, ignoring details for now (would be needed for functional correctness)
+// the first two should be concretely defined (for now in TLSInfo)
 
 let is_stream_ae i = pv_of_id i = TLS_1p3
 let is_stateful_lhae i = pv_of_id i <> TLS_1p3 /\ is_AEAD i.aeAlg /\ ~ (authId i)
 
-// as a temporary hack, we currently disable AuthId for TLS 1.2.
+// NB as a temporary hack, we currently disable AuthId for TLS 1.2.
 // so that we can experiment with TLS and StreamAE
 
+assume val validCipherLen: i:id -> l:nat -> Type0 // sufficient to ensure the cipher can be processed without length errors
+assume val cipherLen: i:id -> fragment i -> Tot (l:nat {validCipherLen i l})
+
+type encipher (#i:id) (f:fragment i) = lbytes (cipherLen i f)
+type decipher (i:id) = b:bytes { validCipherLen i (length b) }
+
+// concrete key materials, for leaking & coercing.
+// (each implementation splits it into encryption keys, IVs, MAC keys, etc)
+
+let aeKeySize (i:id) = 
+  if pv_of_id i = TLS_1p3 
+  then CoreCrypto.aeadKeySize (StreamAE.alg i) + CoreCrypto.aeadRealIVSize (StreamAE.alg i)
+  else 0 //FIXME!
+
+type keybytes (i:id) = lbytes (aeKeySize i)
+
+// abstract instances
 
 type state (i:id) (rw:rw) = 
-  | Stream: u:unit{is_stream_ae i} -> StreamAE.state i rw -> state i rw
+  | Stream: u:unit{is_stream_ae i}         -> StreamAE.state i rw -> state i rw
   | StLHAE: u:unit{is_stateful_lhae i} -> StatefulLHAE.state i rw -> state i rw
 
 type reader i = state i Reader
 type writer i = state i Writer
+
+val region:     #i:id -> #rw:rw -> state i rw -> Tot rgn
+let region (#i:id) (#rw:rw) (s:state i rw): Tot rgn
+  = match s with 
+    | Stream _ s -> StreamAE.State.region s
+    | StLHAE _ s -> StatefulLHAE.region s
+
+val log_region: #i:id -> #rw:rw -> state i rw -> Tot rgn
+let log_region (#i:id) (#rw:rw) (s:state i rw): Tot rgn
+  = match s with 
+    | Stream _ s -> StreamAE.State.log_region s
+    | StLHAE _ s -> if rw = Writer then StatefulLHAE.region s else StatefulLHAE.peer_region s //FIXME
+
+
+// how to specify those two? Their properties are available at creation-time. 
+
+
+// our view to AE's ideal log (when idealized, ignoring ciphers) and counter
+// TODO: write down their joint monotonic specification: both are monotonic, and seqn = length log when ideal
+
+type ideal_log (i:id) = seq (fragment i)  // TODO: consider adding constraint on terminator fragments
+
+// TODO extend library? We need a full spec
+assume val seq_mapT: ('a -> Tot 'b) -> seq 'a -> Tot (seq 'b)
+
+assume val logT: #i:id { authId i } -> #rw:rw -> state i rw -> HH.t -> GTot (ideal_log i)
+(* let logT #i #rw (s:state i rw) h =  *)
+(*   match s with  *)
+(*   | Stream _ s -> let written = m_sel h (StreamAE.State.log s) in  *)
+(*                  let project (StreamAE.Entry #i l c p) (\*: Content.fragment i *\) = p in *)
+(*                  seq_mapT #(StreamAE.entry i) #(fragment i) project written  *)
+
+val seqnT: #i:id -> #rw:rw -> state i rw -> HH.t -> GTot seqn_t 
+let seqnT #i #rw (s:state i rw) h = 
+  match s with 
+  | Stream _ s -> m_sel h (StreamAE.ctr (StreamAE.State.counter s))
+  | StLHAE _ s -> sel h (StatefulLHAE.State.seqn s)
+
+let incrementable (#i:id) (#rw:rw) (s:state i rw) (h:HH.t) = is_seqn (seqnT s h + 1)
 
 let stream_ae (#i:id{is_stream_ae i}) (#rw:rw) (s:state i rw) 
   : Tot (StreamAE.state i rw)
@@ -31,34 +93,14 @@ let st_lhae (#i:id{is_stateful_lhae i}) (#rw:rw) (s:state i rw)
   : Tot (StatefulLHAE.state i rw)
   = let StLHAE _ s = s in s
 
-open FStar.HyperHeap
-type n_rid = r:rid{r <> root}
-
-let region (#i:id) (#rw:rw) (s:state i rw): Tot n_rid
-  = match s with 
-    | Stream _ s -> StreamAE.State.region s
-    | StLHAE _ s -> StatefulLHAE.region s
-
-let log_region (#i:id) (#rw:rw) (s:state i rw): Tot n_rid
-  = match s with 
-    | Stream _ s -> StreamAE.State.log_region s
-    | StLHAE _ s -> StatefulLHAE.peer_region s //FIXME
-
 let writable_seqn (#i:id) (#rw:rw) (s:state i rw) h = 
     match s with 
     | Stream _ s -> is_seqn (m_sel h (StreamAE.ctr (StreamAE.State.counter s)) + 1)
     | StLHAE _ s -> is_seqn (sel h (StatefulLHAE.State.seqn s) + 1) 
 
-(*
-let counter (#i:id { is_stream_ae i }) (#rw:rw) (s:state i rw): Tot seqn_ref s.region i log
-  = match s with 
-    | Stream _ s -> StreamAE.State.counter s
 
-let log (#i:id) (#rw:rw) (s:state i rw) : Tot (StreamAE.log_ref (log_region s) i)
-  = match s with 
-    | Stream _ s -> StreamAE.State.log_region s
-    | StLHAE _ s -> ()
-*)
+(*
+
 type cipher (i:id) = b:bytes {Range.valid_clen i (length b)}
 
 let cipher_noId b : cipher noId = b 
@@ -80,3 +122,97 @@ let writer_modifies #i h0 wr h1 =
       HyperHeap.modifies (Set.singleton (StatefulLHAE.region wr)) h0 h1 /\
       Heap.modifies (!{ as_ref (StatefulLHAE.log wr), as_ref (StatefulLHAE.seqn wr)}) (Map.sel h0 (StatefulLHAE.region wr)) (Map.sel h1 (StatefulLHAE.region wr)) )
 
+*)
+
+
+
+// Some invariants:
+// - the writer counter is the length of the log; the reader counter is lower or equal
+// - gen is called at most once for each (i:id), generating distinct refs for each (i:id)
+// - the log is monotonic
+
+// We generate first the writer, then the reader (possibly several of them)
+
+let genPost (#i:id) parent h0 (w:writer i) h1 = 
+  let r = region w in 
+  modifies Set.empty h0 h1 /\
+  HH.parent r = parent /\
+  fresh_region r h0 h1 /\
+  color r = color parent /\
+  seqnT w h1 = 0 /\
+  (authId i ==> logT #i #Writer w h1 = createEmpty) // we need to re-apply #i knowning authId
+
+// Generate a fresh instance with index i in a fresh sub-region 
+
+assume val gen: parent:rid -> i:id -> ST (writer i)
+  (requires (fun h0 -> True))
+  (ensures (genPost parent))
+
+// Coerce a writer with index i in a fresh subregion of parent
+// (coerced readers can then be obtained by calling genReader)
+assume val coerce: parent:rid -> i:id{~(authId i)} -> keybytes i -> ST (writer i)
+  (requires (fun h0 -> True))
+  (ensures  (genPost parent))
+
+assume val leak: #i:id{~(authId i)} -> #role:rw -> state i role -> ST (keybytes i)
+  (requires (fun h0 -> True))
+  (ensures  (fun h0 r h1 -> modifies Set.empty h0 h1 ))
+
+assume val genReader: parent:rid -> #i:id -> w:writer i -> ST (reader i)
+  (requires (fun h0 -> HyperHeap.disjoint parent (region w))) //16-04-25  we may need w.region's parent instead
+  (ensures  (fun h0 (r:reader i) h1 ->
+               modifies Set.empty h0 h1 /\
+               log_region r = region w /\
+               HH.parent (region r) = parent /\
+	       color (region r) = color parent /\
+               fresh_region (region r ) h0 h1 /\
+               //?? op_Equality #(log_ref w.region i) w.log r.log /\
+               seqnT r h1 = 0))
+// encryption, recorded in the log; safe instances are idealized
+assume val encrypt: #i:id -> e:writer i -> f:fragment i -> ST (encipher f)
+  (requires (fun h0 -> incrementable e h0))
+  (ensures  (fun h0 c h1 ->
+               modifies_one (region e) h0 h1 /\
+               seqnT e h1 = seqnT e h0 + 1 /\
+               authId i ==> logT #i #Writer e h1 = SeqProperties.snoc (logT #i #Writer e h0) f))
+//TODO restore monotonic post; see StreamAE.fsti
+
+// decryption, idealized as a lookup for safe instances
+assume val decrypt: #i:id -> d:reader i -> c:decipher i -> ST (option (f:fragment i { length c = cipherLen i f}))
+  (requires (fun h0 -> incrementable d h0))
+  (ensures  (fun h0 res h1 ->
+	      match res with
+ 	     | None   -> modifies Set.empty h0 h1
+	     | Some f -> let j = seqnT d h0 in 
+                        modifies_one (region d) h0 h1 /\ 
+                        seqnT d h1 = j + 1 /\
+                        (authId i ==>
+                           (let written = logT #i #Reader d h1 in 
+                           j < Seq.length written /\
+                           f = Seq.index written j)))) 
+
+
+(* let gen parent i =  *)
+(*   assert(is_stream_ae i);  *)
+(*   Stream(StreamAE.gen parent i) *)
+
+(* let coerce parent i kiv =  *)
+(*   assert(is_stream_ae i);  *)
+(*   let kv, iv = split kiv (CoreCrypto.aeadKeySize (StreamAE.alg i)) in *)
+(*   Stream(StreamAE.coerce parent i kv iv) *)
+
+(* let leak #i #role s =  *)
+(*   assert(is_stream_ae i);  *)
+(*   StreamAE.leak s  *)
+
+(* let genReader parent w i =  *)
+(*   assert(is_stream_ae i);  *)
+(*   Stream(StreamAE.genReader parent i w) *)
+
+(* let encrypt #i e f =  *)
+(*   match e with *)
+(*   | Stream _ s -> StreamAE.encrypt s f *)
+
+(* let decrypt #i d c =  *)
+(*   match d with *)
+(*   | Stream _ s -> StreamAE.decrypt s c *)
